Cleanup

racket/induction.rkt
@@ -1,0 +1,60 @@
+;;; Some examples of using Rosette to verify hardware designs.
+
+#lang rosette
+
+(require rosette/lib/synthax)
+(require "utils.rkt")
+
+(define (interpret prog env id time cache bitwidth)
+  (if (< time 0) (error 'interpret "time must be non-negative") 0)
+  (match (list-ref prog id)
+    [`(Var ,x)
+     (begin
+       (when (not (symbol? x))
+         (error 'interpret "expected a symbol"))
+       (hash-ref env x))]
+    [`(Op ,op ,ids ...)
+     (apply op
+            (for/list ([id ids])
+              (interpret prog env id time cache bitwidth)))]
+    [`(Reg ,reg-id ,init)
+     (displayln (format "time is ~a" time))
+     (if (= time 0)
+         init
+         (if (hash-has-key? cache (- time 1))
+             (hash-ref cache (- time 1))
+             (interpret prog env reg-id (- time 1) cache bitwidth)))]
+    [node
+     (begin
+       (when (not (bv? node))
+         (error 'interpret "expected a bitvector"))
+       node)]))
+
+;;; use rosette to verify that the program always evaluates to 1
+(define prog (list `(Reg ,0 ,(bv 1 1))))
+(define-symbolic t integer?)
+
+(define cache (make-hash))
+
+(verify (begin
+          (hash-set! cache (- t 1) (bv 1 1))
+          (assume (>= t 0))
+          (assert (bveq (interpret prog '() 0 t cache 1) (bv 1 1)))))
+
+(clear-vc!)
+
+;;; counter[2] at time t is (t + 1)
+(define counter (list `(Reg ,2 ,(bv 0 10)) (bv 1 10) `(Op ,bvadd ,0 ,1)))
+
+;;; clear the cache
+(define new-cache (make-hash))
+
+(define-symbolic result (bitvector 10))
+
+(verify (begin
+          (assume (bveq result (integer->bitvector t (bitvector 10))))
+          (assume (> t 0))
+          (hash-set! new-cache t result)
+          (assert (bveq (interpret counter '() 2 0 new-cache 10) (bv 1 10)))
+          (assert (bveq (interpret counter '() 2 (+ t 1) new-cache 10)
+                        (integer->bitvector (+ t 1) (bitvector 10))))))
