racket/min-example.rkt
@@ -1,0 +1,25 @@
+#lang rosette
+
+(define (identity t)
+  (displayln (format "t is ~a" t))
+  (if (zero? t) 0 (+ 1 (identity (- t 1)))))
+
+(define (cached-identity t cache)
+  (if (zero? t)
+      0
+      (if (hash-has-key? cache t) (hash-ref cache t) (+ 1 (cached-identity (- t 1) cache)))))
+
+(define-symbolic t integer?)
+
+;;; this won't terminate
+;;; (verify (begin
+;;;           (assume (>= t 0))
+;;;           (assert (= (identity t) t))))
+
+;;; this will terminate
+(define cache (make-hash))
+
+(verify (begin
+          (hash-set! cache t t)
+          (assume (> t 0))
+          (assert (= (cached-identity (+ t 10) cache) (+ t 10)))))
